thys/Interpreter_Optimizations/Std.thy
@@ -1,5 +1,5 @@
 theory Std
-  imports List_util Global Op Env Env_list Dynamic
+  imports List_util Global Op Env Dynamic
     "VeriComp.Language"
 begin
 
@@ -115,10 +115,7 @@ proof (rule notI)
   then obtain s' where "step s s'" by auto
   thus False
     using \<open>final F_get IReturn s\<close>
-    by (auto
-        simp: state_ok_def
-          wf_fundefs_imp_wf_fundef[THEN wf_fundef_last_basic_block, THEN next_instr_length_instrs[rotated]]
-        elim!: step.cases final.cases)
+    by (auto simp: state_ok_def elim!: step.cases final.cases)
 qed
 
 sublocale semantics step "final F_get IReturn"
